Loosen the bounds for splitting a segment
Previously the split point could not be at the very beginning or very
end of a segment. This seems to make sense (it's certainly a degenerate
case) but without this capability we can't use induction on segments
with length = 2.

AngelDevil/Segment.lean
@@ -37,7 +37,7 @@ structure TraceSegment where
   blocked : List (Int × Int)
   i : Nat
   j : Nat
-  ilt : i < j
+  ile : i ≤ j
   jlt : j < (trace n start blocked).length
 
 -- Get the underlying trace on which the segment is based
@@ -45,7 +45,7 @@ def segment_trace (seg : TraceSegment) : List RunState := trace seg.n seg.start 
 
 -- Get the first RunState of the segment
 def segment_start (seg : TraceSegment) : RunState :=
-  (segment_trace seg)[seg.i]'(lt_trans seg.ilt seg.jlt)
+  (segment_trace seg)[seg.i]'(lt_of_le_of_lt seg.ile seg.jlt)
 
 -- Get the last RunState of the segment
 def segment_end (seg : TraceSegment) : RunState :=
@@ -59,23 +59,23 @@ def segment_states (seg : TraceSegment) : List RunState :=
 def segment_length (seg : TraceSegment) : Nat := seg.j - seg.i + 1
 
 -- Split the segment into two pieces and take the first part
-def segment_split_first (seg : TraceSegment) (k : Nat) (ltk : seg.i < k) (klt : k < seg.j) : TraceSegment where
+def segment_split_first (seg : TraceSegment) (k : Nat) (lek : seg.i ≤ k) (kle : k ≤ seg.j) : TraceSegment where
   n := seg.n
   start := seg.start
   blocked := seg.blocked
   i := seg.i
   j := k
-  ilt := ltk
-  jlt := lt_trans klt seg.jlt
+  ile := lek
+  jlt := lt_of_le_of_lt kle seg.jlt
 
 -- Split the segment into two pieces and take the second part
-def segment_split_second (seg : TraceSegment) (k : Nat) (_ : seg.i < k) (klt : k < seg.j) : TraceSegment where
+def segment_split_second (seg : TraceSegment) (k : Nat) (_ : seg.i ≤ k) (kle : k ≤ seg.j) : TraceSegment where
   n := seg.n
   start := seg.start
   blocked := seg.blocked
   i := k
   j := seg.j
-  ilt := klt
+  ile := kle
   jlt := seg.jlt
 
 -- The length of the segment states is the same as the segment length
@@ -84,104 +84,104 @@ lemma segment_states_length (seg : TraceSegment) :
   unfold segment_states segment_trace segment_length
   rw [List.length_take_of_le]
   rw [List.length_drop, trace_length]
-  apply Nat.add_one_le_of_lt (Nat.sub_lt_sub_right (le_of_lt seg.ilt) _)
+  apply Nat.add_one_le_of_lt (Nat.sub_lt_sub_right seg.ile _)
   apply (trace_length _ _ _) ▸ seg.jlt
 
 -- Get the length of the first half of a split trace
-lemma segment_split_first_length (seg : TraceSegment) (k : Nat) (ltk : seg.i < k) (klt : k < seg.j) :
-  segment_length (segment_split_first seg k ltk klt) = k - seg.i + 1 := by
+lemma segment_split_first_length (seg : TraceSegment) (k : Nat) (lek : seg.i ≤ k) (kle : k ≤ seg.j) :
+  segment_length (segment_split_first seg k lek kle) = k - seg.i + 1 := by
   unfold segment_length segment_split_first; simp
 
 -- Get the length of the second half of a split trace
-lemma segment_split_second_length (seg : TraceSegment) (k : Nat) (ltk : seg.i < k) (klt : k < seg.j) :
-  segment_length (segment_split_second seg k ltk klt) = seg.j - k + 1 := by
+lemma segment_split_second_length (seg : TraceSegment) (k : Nat) (lek : seg.i ≤ k) (kle : k ≤ seg.j) :
+  segment_length (segment_split_second seg k lek kle) = seg.j - k + 1 := by
   unfold segment_length segment_split_second; simp
 
 -- The length of a segment is one less than the sum of the
 -- lengths of its two parts
-lemma segment_split_length (seg : TraceSegment) (k : Nat) (ltk : seg.i < k) (klt : k < seg.j) :
+lemma segment_split_length (seg : TraceSegment) (k : Nat) (lek : seg.i ≤ k) (kle : k ≤ seg.j) :
   segment_length seg =
-  (segment_length (segment_split_first seg k ltk klt)) +
-  (segment_length (segment_split_second seg k ltk klt)) - 1 := by
+  (segment_length (segment_split_first seg k lek kle)) +
+  (segment_length (segment_split_second seg k lek kle)) - 1 := by
   rw [segment_split_first_length, segment_split_second_length, segment_length]; simp
-  rw [add_comm _ (seg.j - k), ← add_assoc, ← Nat.add_sub_assoc (le_of_lt ltk)]
-  rw [Nat.sub_add_cancel (le_of_lt klt)]
+  rw [add_comm _ (seg.j - k), ← add_assoc, ← Nat.add_sub_assoc lek]
+  rw [Nat.sub_add_cancel kle]
 
 -- Get an element from the first half of a split trace segment
 lemma segment_split_first_states_getElem
-  (seg : TraceSegment) (k : Nat) (ltk : seg.i < k) (klt : k < seg.j) :
-  ∀ a (alt : a < (segment_states (segment_split_first seg k ltk klt)).length),
-  (segment_states (segment_split_first seg k ltk klt))[a] =
+  (seg : TraceSegment) (k : Nat) (lek : seg.i ≤ k) (kle : k ≤ seg.j) :
+  ∀ a (alt : a < (segment_states (segment_split_first seg k lek kle)).length),
+  (segment_states (segment_split_first seg k lek kle))[a] =
   (segment_states seg)[a]'(by
     rw [segment_states_length, segment_split_first_length] at alt
     rw [segment_states_length, segment_length]
-    exact lt_trans alt ((Nat.add_lt_add_right (Nat.sub_lt_sub_right (le_of_lt ltk) klt)) _)
+    exact lt_of_lt_of_le alt ((Nat.add_le_add_right (Nat.sub_le_sub_right kle _)) _)
   ) := by
   intro _ _
   unfold segment_states segment_split_first segment_trace; simp
 
 -- Get an element from the second half of a split trace segment
 lemma segment_split_second_states_getElem
-  (seg : TraceSegment) (k : Nat) (ltk : seg.i < k) (klt : k < seg.j) :
-  ∀ a (alt : a < (segment_states (segment_split_second seg k ltk klt)).length),
-  (segment_states (segment_split_second seg k ltk klt))[a] =
+  (seg : TraceSegment) (k : Nat) (lek : seg.i ≤ k) (kle : k ≤ seg.j) :
+  ∀ a (alt : a < (segment_states (segment_split_second seg k lek kle)).length),
+  (segment_states (segment_split_second seg k lek kle))[a] =
   (segment_states seg)[a + k - seg.i]'(by
     rw [segment_states_length, segment_split_second_length] at alt
     rw [segment_states_length, segment_length]
-    apply Nat.sub_lt_right_of_lt_add (le_of_lt (lt_of_lt_of_le ltk (Nat.le_add_left _ _)))
+    apply Nat.sub_lt_right_of_lt_add (le_trans lek (Nat.le_add_left _ _))
     rw [add_right_comm, Nat.sub_add_cancel]; swap
-    · exact le_of_lt (lt_trans ltk klt)
+    · exact le_trans lek kle
     apply Nat.add_lt_of_lt_sub
     rwa [Nat.sub_add_comm]
-    exact le_of_lt klt
+    exact kle
   ) := by
   intro a alt
   unfold segment_states segment_split_second segment_trace; simp; congr 1
   rw [add_comm, add_comm seg.i, Nat.sub_add_cancel]
-  exact le_of_lt (lt_of_lt_of_le ltk (Nat.le_add_left _ _))
+  exact le_trans lek (Nat.le_add_left _ _)
 
 -- Prove an identity for the states of the first half of a split segment
-lemma segment_split_first_states (seg : TraceSegment) (k : Nat) (ltk : seg.i < k) (klt : k < seg.j) :
-  segment_states (segment_split_first seg k ltk klt) =
+lemma segment_split_first_states (seg : TraceSegment) (k : Nat) (lek : seg.i ≤ k) (kle : k ≤ seg.j) :
+  segment_states (segment_split_first seg k lek kle) =
   List.take (k - seg.i + 1) (segment_states seg) := by
   apply List.ext_getElem
   · rw [segment_states_length, segment_split_first_length]
     rw [List.length_take_of_le]
     rw [segment_states_length, segment_length]
-    exact Nat.add_le_add_right (Nat.sub_le_sub_right (le_of_lt klt) _) _
+    exact Nat.add_le_add_right (Nat.sub_le_sub_right kle _) _
   intro a alt alt'
   rw [segment_split_first_states_getElem, List.getElem_take]
 
 -- Prove an identity for the states of the second half of a split segment
-lemma segment_split_second_states (seg : TraceSegment) (k : Nat) (ltk : seg.i < k) (klt : k < seg.j) :
-  segment_states (segment_split_second seg k ltk klt) =
+lemma segment_split_second_states (seg : TraceSegment) (k : Nat) (lek : seg.i ≤ k) (kle : k ≤ seg.j) :
+  segment_states (segment_split_second seg k lek kle) =
   List.drop (k - seg.i) (segment_states seg) := by
   apply List.ext_getElem
   · rw [segment_states_length, segment_split_second_length, List.length_drop]
     rw [segment_states_length, segment_length]
-    rw [Nat.sub_sub_right _ (le_of_lt ltk), add_right_comm _ 1]
-    rw [Nat.sub_add_cancel (le_of_lt (lt_trans ltk klt))]
+    rw [Nat.sub_sub_right _ lek, add_right_comm _ 1]
+    rw [Nat.sub_add_cancel (le_trans lek kle)]
     rw [Nat.sub_add_comm]
-    exact le_of_lt klt
+    exact kle
   intro a alt _
   rw [segment_split_second_states_getElem, List.getElem_drop]; congr
   rw [add_comm (k - seg.i), Nat.add_sub_assoc]
-  exact le_of_lt ltk
+  exact lek
 
 -- The list of states for a split segment is equal to those
 -- in the first part followed by the tail of those in the second
-lemma segment_split_states (seg : TraceSegment) (k : Nat) (ltk : seg.i < k) (klt : k < seg.j) :
+lemma segment_split_states (seg : TraceSegment) (k : Nat) (lek : seg.i ≤ k) (kle : k ≤ seg.j) :
   segment_states seg =
-  segment_states (segment_split_first seg k ltk klt) ++
-  (segment_states (segment_split_second seg k ltk klt)).tail := by
+  segment_states (segment_split_first seg k lek kle) ++
+  (segment_states (segment_split_second seg k lek kle)).tail := by
   apply List.ext_getElem
   · rw [List.length_append, List.length_tail, ← Nat.add_sub_assoc]; swap
     · rw [segment_states_length]
       unfold segment_length segment_split_second; simp
     repeat rw [segment_states_length]
-    exact segment_split_length seg k ltk klt
+    exact segment_split_length seg k lek kle
   intro a alt _
-  by_cases alt' : a < (segment_states (segment_split_first seg k ltk klt)).length
+  by_cases alt' : a < (segment_states (segment_split_first seg k lek kle)).length
   · rw [List.getElem_append_left alt']
     rw [segment_split_first_states_getElem]
   · rename' alt' => lea; push_neg at lea
@@ -191,6 +191,6 @@ lemma segment_split_states (seg : TraceSegment) (k : Nat) (ltk : seg.i < k) (klt
     rw [segment_states_length, segment_split_first_length]
     rw [add_assoc, Nat.add_sub_assoc, add_comm 1]; swap
     · rw [add_comm]
-      exact le_of_lt (lt_trans ltk (Nat.lt_add_one _))
-    rw [Nat.sub_add_comm (le_of_lt ltk), Nat.sub_add_cancel]
+      exact le_of_lt (lt_of_le_of_lt lek (Nat.lt_add_one _))
+    rw [Nat.sub_add_comm lek, Nat.sub_add_cancel]
     rwa [segment_states_length, segment_split_first_length] at lea
